proof/correctness/W16extra.ec
@@ -1,119 +1,51 @@
 require import AllCore List IntDiv CoreMap IntDiv.
 from Jasmin require  import JModel JMemory.
+import W16.
 
-op b16 (a : W16.t) (b : int) = 
-     -b <= to_sint a < b axiomatized by b16E.
+op b16 (a : W16.t) (b : int) = -b <= to_sint a < b axiomatized by b16E.
 
-op bpos16 (a : W16.t) (b : int) = 
-     0 <= to_sint a < b  axiomatized by bpos16E.
+op bpos16 (a : W16.t) (b : int) = 0 <= to_sint a < b  axiomatized by bpos16E.
 
-op bw16 (a : W16.t) i =
-     -2^i <= to_sint a < 2^i  axiomatized by bw16E.
+op bw16 (a : W16.t) i = -2^i <= to_sint a < 2^i  axiomatized by bw16E.
 
 hint simplify b16E.
 hint simplify bpos16E.
 hint simplify bw16E.
 
-
-lemma to_sint_unsigned (x : W16.t): 0 <= to_sint x => to_sint x = to_uint x.
-proof. 
-rewrite W16.to_sintE /smod.
-move : (W16.to_uint_cmp x) => /> ? ?.
-case (32768 <= to_uint x) => ? // /#. 
-qed.
+lemma to_sint_unsigned (x : W16.t): 0 <= to_sint x => to_sint x = to_uint x 
+   by smt(to_sintE to_uint_cmp).
 
 lemma to_sintD_small (a b : W16.t):
 -W16.modulus %/2 <= to_sint a + to_sint b < W16.modulus %/2 =>
-to_sint (a + b) = to_sint a + to_sint b.
-proof. 
-rewrite !W16.to_sintE !/smod => />.
-move : (W16.to_uint_cmp a) (W16.to_uint_cmp b) => /> *.
-have sumbnd : to_uint a + to_uint b < 65536+65536 ; first  by auto => /#. 
-case (65536  <= to_uint a + to_uint b).
-+   move => *; rewrite (_:  to_uint (a + b)= (to_uint a +  to_uint b) - 65536);
-       [rewrite to_uintD => /> /# | auto => /#].
-+    move => *; rewrite (_:  to_uint (a + b)= (to_uint a +  to_uint b));
-       [rewrite to_uintD_small => /> /# |  auto => /#].
-qed.
-
+      to_sint (a + b) = to_sint a + to_sint b
+  by rewrite !to_sintE /smod /= to_uintD;smt(to_uint_cmp).
 
 lemma to_sintB_small(a b : W16.t):
     -W16.modulus %/2 <= to_sint a - to_sint b < W16.modulus %/2 =>
-    to_sint (a - b) = to_sint a - to_sint b.
-proof.
-rewrite !W16.to_sintE !/smod => />.
-move : (W16.to_uint_cmp a) (W16.to_uint_cmp b) => />. 
-case (to_uint b <= to_uint a).
-+ case(32768 <= to_uint a);
-    move =>*;
-    rewrite (_:  to_uint (a - b)= (to_uint a -  to_uint b));
-     [ rewrite to_uintD to_uintN modzDmr => /> /# | auto => /> /#|
-       rewrite to_uintD to_uintN modzDmr => /> /# | auto => /> /#].
-+ case(32768 <= to_uint a);
-    move =>*;
-    rewrite (_:  to_uint (a - b)= (to_uint a -  to_uint b) + 65536);
-     [ rewrite to_uintD to_uintN modzDmr => /> /# | auto => /> /#|
-       rewrite to_uintD to_uintN modzDmr => /> /# | auto => /> /#].
-qed.
+          to_sint (a - b) = to_sint a - to_sint b
+ by rewrite !W16.to_sintE !/smod /= to_uintD to_uintN modzDmr; smt(to_uint_cmp).
 
 lemma to_sintb_lt0(x y : W16.t): 
     0 <= to_sint x =>
     0 <= to_sint y =>
     to_sint (x - y) < 0 => to_sint x < to_sint y.
 proof.
-rewrite W16.to_sintE /smod.
-move : (W16.to_uint_cmp x) => /> ? ?.
-case (32768 <= to_uint x) => ? // ?H5 H6; first by smt().
-move : H5;rewrite W16.to_sintE /smod.
-move : (W16.to_uint_cmp y) => /> ? ?.
-case (32768 <= to_uint y) => ? //; first by smt().
-move : H6; rewrite to_sintB_small !to_sintE /smod => /#.
-qed.
-
-
-lemma aux xx yy : 
-! 32768 <= yy =>
-32768 <= xx =>
-0 <= xx =>
-xx < 65536 =>
-0 <= yy =>
-yy < 65536 =>
--32768 <= (xx - 65536) * yy =>
-(xx - 65536) * yy < 32768 =>
-(if 32768 <= xx * yy %% 65536 then xx * yy %% 65536 - 65536
- else xx * yy %% 65536) =
-(xx - 65536) * yy.
-proof. 
-move => *. 
-case (yy = 0); first by smt().
-case (yy = 1); first by smt().
-move => *.
-have ? : (32768 <= xx * yy %% 65536); by auto => /> /#.
+rewrite (to_sintE x) (to_sintE y) /smod /=.
+move : (to_uint_cmp x)  (to_uint_cmp y) => /=.
+case (32768 <= to_uint x); 1: by smt(). 
+case (32768 <= to_uint y); 1: by smt(). 
+by move => b1 b2 xl xh yl yh; rewrite to_sintB_small /=;
+  rewrite!to_sintE /smod /=; smt().
 qed.
 
 lemma to_sintM_small(a b : W16.t): 
     -W16.modulus %/2 <= to_sint a * to_sint b < W16.modulus %/2 =>
     to_sint (a * b) = to_sint a * to_sint b.
 proof.
-rewrite !W16.to_sintE !/smod => />.
-move : (W16.to_uint_cmp a) (W16.to_uint_cmp b) => />.
-rewrite to_uintM => />. 
-pose xx := to_uint a.
-pose yy := to_uint b.
-case(32768 <= xx); last first. 
-case(32768 <= yy); last first. 
-+ smt(@Int @IntDiv).
-+ move => /> *; rewrite mulzC (mulzC xx (yy-65536));apply (aux yy xx) => /#.
-case(32768 <= yy); first by smt(). 
-apply (aux xx yy) => /#.   
+rewrite !to_sintE !/smod /= to_uintM /=. 
+by case(32768 <= to_uint a); case(32768 <= to_uint b);  smt(). 
 qed.
 
 lemma to_sintN (a : W16.t) : 
--W16.modulus %/2 < to_sint a < W16.modulus %/2 => to_sint (- a) = - to_sint a.
-proof. 
-rewrite !to_sintE /smod !to_uintN=> /> *. 
-move : (W16.to_uint_cmp a) => /> *. 
-case (to_uint a = 0); first by smt().
-case (to_uint a = 65535); first by smt().
-by move => *; rewrite (_: (- to_uint a) %% 65536 = 65536 - to_uint a) => /> /#.
-qed.
+-W16.modulus %/2 < to_sint a < W16.modulus %/2 => to_sint (- a) = - to_sint a
+   by rewrite !to_sintE /smod !to_uintN /=; smt(to_uint_cmp).
